---
title: "Homework 3 (Part 1)"
author: "Michael Pena"
date: "2024-02-17"
output: pdf_document
packages:
  - bm
---

```{r setup, include=FALSE}
knitr::opts_chunk$set(echo = TRUE)
```

# Part (a)

$$
\partial \ell (\partial \mathbf{\mu}) = Tr \Bigl(\mathbf{\Sigma^{-1}} \sum^{n}_{i=1}\partial \mathbf{\mu}(\mathbf{x}_i - \mathbf{\mu})^T\Bigl)
$$

the ith element will be $\Big[ \mathbf{\Sigma^{-1}} \sum^{n}_{i=1}(\mathbf{x}_i - \mathbf{\mu})\Big]_i$


$$
\partial \ell (\partial \mathbf{\Sigma}) = \frac{-n}{2}Tr\Bigl(
\mathbf{\Sigma}^{-1} (\mathbf{\Sigma} - \frac{C(\mathbf{\mu})}{2})\mathbf{\Sigma}^{-1} \partial \mathbf{\Sigma}
\Bigl)
$$
here let $A = \mathbf{\Sigma}^{-1}(\mathbf{\Sigma} - \frac{C(\mathbf{\mu})}{n})\mathbf{\Sigma}^{-1}$

when $i = j$
$$
\frac{\partial \ell}{\partial \sigma_{ij}} = 
\frac{-n}{2}A_{ii}
$$

when $i \ne j$
$$
\frac{\partial \ell}{\partial \sigma_{ij}} = 
\frac{-n}{2}(A_{ij} + A_{ji}) 
$$

$$
\partial^2 \ell (\partial \mathbf{\mu} \partial \mathbf{\mu}) = 
-Tr \Bigl( -\mathbf{\Sigma}^{-1} n \partial \mathbf{\mu} \partial \mathbf{\mu}^T 
\Bigl)
$$

nonzero when $i \ne j$
$$
\frac{\partial^2 \ell}{\partial \mu_i \partial \mu_j} = 
-n\Sigma^{-1}_{ij}
$$


$$
\partial^2 \ell (\partial \mathbf{\mu} \partial \mathbf{\Sigma}) = 
Tr \Bigl(
(-\mathbf{\Sigma}^{-1}(\partial \mathbf{\Sigma}) \mathbf{\Sigma}^{-1}) \sum^{n}_{i=1}\partial \mathbf{\mu}(\mathbf{x}_i - \mu)^T
\Bigl)
$$

when $i=j$
$$
\frac{\partial^2\ell}{\partial \mu_k \partial \sigma_{ij}} = 
-\sum^{p}_{n=1}\Bigl[
\Sigma^{-1}_{in} \Sigma^{-1}_{ki}
\Big(\sum^{m}_{z=1} (x_z - \mu)^T
\Big) 
\Bigl]
$$

when $i \ne  j$
$$
\frac{\partial^2\ell}{\partial \mu_k \partial \sigma_{ij}} = 
-\sum^{p}_{n=1}\Bigl[
\Big(
\Sigma^{-1}_{in} \Sigma^{-1}_{kj} +
\Sigma^{-1}_{jn} \Sigma^{-1}_{ki}
\Big)
\Big(\sum^{m}_{z=1} (x_z - \mu)^T
\Big) 
\Bigl]
$$

$$
\partial^2 \ell (\partial \mathbf{\Sigma} \partial \mathbf{\Sigma})=
n Tr \Bigl(
\mathbf{\Sigma}^{-1}(\mathbf{\Sigma} - \frac{C(\mu)}{n} + \frac{1}{2}I) \mathbf{\Sigma}^{-1} \partial \mathbf{\Sigma} \mathbf{\Sigma}^{-1} \partial \mathbf{\Sigma} 
\Bigl)
$$

let $A = \mathbf{\Sigma}^{-1}(\mathbf{\Sigma} - \frac{C(\mu)}{n} + \frac{1}{2}I) \mathbf{\Sigma}^{-1}$

when $i=j,k=l$
$$
\frac{\partial^2\ell}{\partial \sigma_{ij} \partial \sigma_{kl}} =
\frac{n}{2}A_{ki}\Sigma^{-1}_{ik}
$$

when $i \neq j, k = l$
$$
\frac{\partial^2\ell}{\partial \sigma_{ij} \partial \sigma_{kl}} =
\frac{n}{2} \Bigr[
A_{kj}[\Sigma^{-1}]_{il} +
A_{ki}[\Sigma^{-1}]_{jl} 
\Bigr]
$$ 

when $i = j, k \neq l$
$$
\frac{\partial^2 \ell}{\partial \sigma_{ij} \partial \sigma_{kl}} = 
\frac{n}{2} \Bigr[
A_{kj}[\Sigma^{-1}]_{il} +
A_{li}[\Sigma^{-1}]_{ik}
\Bigr]
$$

when $i\ne j, k\ne l$
$$
\frac{\partial^2\ell}{\partial \sigma_{ij} \partial \sigma_{kl}} =
\frac{n}{2} \Bigr[
A_{kj}[\Sigma^{-1}]_{il} +
A_{ki}[\Sigma^{-1}]_{jl} +
A_{lj}[\Sigma^{-1}]_{ik} +
A_{li}[\Sigma^{-1}]_{jk}
\Bigr]
$$



## Part (b)

we know that $E[\Sigma^{-1}]= \Sigma^{-1}$ and $E[x_i - \mu] = 0$
when considering $E[\frac{\partial^2 \ell}{\partial \sigma_{ij} \partial \mu_{k}}]$ both cases have $\sum^{n}_{i=1}(x_i - \mu)$ being multiplied thus both cases are zero.


when considering $E[\frac{\partial^2 \ell}{\partial \mu_{ij} \partial \mu_{ij}}]$

$i \neq j$ case
$$
E[\frac{\partial^2 \ell}{\partial \mu_{i} \partial \mu_{i}}] = 
n[\Sigma^{-1}]_{ij} 
$$


when considering $E[\frac{\partial^2 \ell}{\partial \sigma_{ij} \partial \sigma_{kl}}]$
we know that 

when $i=j,k=l$
$$
E[\frac{\partial^2 \ell}{\partial \sigma_{ij} \partial \sigma_{kl}}] = 
\frac{n}{2}\Sigma^{-1}_{ki}\Sigma^{-1}_{ik}
$$

when $i \neq j, k = l$
$$
E[\frac{\partial^2 \ell}{\partial \sigma_{ij} \partial \sigma_{kl}}] = 
\frac{n}{2} \Bigr[
\Sigma^{-1}_{kj}[\Sigma^{-1}]_{il} +
\Sigma^{-1}_{ki}[\Sigma^{-1}]_{jl} 
\Bigr]
$$

when $i = j, k \neq l$
$$
E[\frac{\partial^2 \ell}{\partial \sigma_{ij} \partial \sigma_{kl}}] = 
\frac{n}{2} \Bigr[
\Sigma^{-1}_{kj}[\Sigma^{-1}]_{il} +
\Sigma^{-1}_{li}[\Sigma^{-1}]_{ik}
\Bigr]
$$

when $i \neq j, k \neq l$
$$
E[\frac{\partial^2 \ell}{\partial \sigma_{ij} \partial \sigma_{kl}}] = 
\frac{n}{2} \Bigr[
\Sigma^{-1}_{kj}[\Sigma^{-1}]_{il} +
\Sigma^{-1}_{ki}[\Sigma^{-1}]_{jl} +
\Sigma^{-1}_{lj}[\Sigma^{-1}]_{ik} +
\Sigma^{-1}_{li}[\Sigma^{-1}]_{jk}
\Bigr]
$$